src/lang/lemmas.v
@@ -207,3 +207,23 @@ Proof.
     simpl in *.
     destruct x; try done.
 Qed.
+
+Lemma prim_step_flush_no_fork ℓ SV PV BV (σ1 : state nvm_lang)
+  (g1 : global_state nvm_lang) (κ : list (language.observation nvm_lang))
+  (e2 : language.expr nvm_lang) (σ2 : state nvm_lang) (g2 : global_state nvm_lang)
+  (efs : list (language.expr nvm_lang)) :
+  prim_step (Flush #ℓ `at` (SV, PV, BV)) σ1 g1 κ e2 σ2 g2 efs → efs = [].
+Proof.
+    intros [Ki [??] [??] ? ? step].
+    subst.
+    simpl in *.
+    induction Ki using rev_ind.
+    { simpl in *. subst. inv_impure_thread_step; try done.
+      rewrite list_fmap_singleton.
+      subst.
+      congruence. }
+    move: H.
+    rewrite fill_app.
+    simpl.
+    destruct x; try done.
+Qed.
